proof of the linkable correctness property for cps conversion.
there are 2 admits. one of them is trivial.
the other needs a change in L5.eval_c:
need to add rule(s) to ensure that
for all values v, eval_c v v.

(note to self: this work was done few weeks ago (branch cpsLinkableMerged)).

certicoq/theories/L4_deBruijn/instances.v
@@ -289,9 +289,8 @@ Global Instance ObsSubtermTermL5 : ObserveNthSubterm (ienv * L5Term) :=
 
 Global Instance certiL5: CerticoqLanguage (ienv * L5Term) := {}.
 
-Definition haltCont : L5Term := KLam_c contVar (Halt_c (vterm contVar)).
 
-Lemma haltContAp t : eval_c (Ret_c haltCont t) t.
+Lemma haltContAp (t: L5Term):  eval_c (Ret_c haltCont t) t.
 Proof.
   unfold haltCont.
   rewrite eval_ret.
@@ -320,7 +319,7 @@ Lemma valueObsEq (senv: ienv) : forall (sv:L4_5_Term), is_value sv ->
                                                   (senv, sv) ⊑ (senv, cps_cvt_val sv).
 Proof using.
   intros ? Hisv.
-  induction Hisv; simpl.
+  induction Hisv; simpl. (* this is proof by induction, not coinduction *)
 - constructor; compute; intros qn; [ destruct qn | ]; constructor.
 - constructor; compute; intros qn; [ destruct qn | ]; constructor.
 - constructor.
@@ -338,16 +337,41 @@ Qed.
                                                   
 Require Import L4.variables.
 Require Import L4.varInterface.
-Global Instance certiL4_5_to_L5Correct: CerticoqTranslationCorrect certiL4_5 certiL5.
-Proof.
-  constructor.
-- simpl. red. intros ? Hgood.
+
+
+  Hint Unfold certiClasses.translate liftTotal bigStepEval certiClasses.bigStepEval
+       liftBigStepException translateT certiL4_5_to_L5  bigStepEval dummyEnvBigStep
+       yesPreserved questionHead QuestionHeadTermL45 QuestionHeadTermL5
+       BigStepOpSem_instance_1  BigStepOpSem_instance_0
+       goodTerm dummyEnvWf goodTerm GoodTerm_instance_0
+       GoodTerm_instance_1: certiclasses.
+
+  Require Import Morphisms.
+Global Instance evalPreservesGood :
+  Proper (eval ==> Basics.impl) (@goodTerm L4_5_Term _).
+Proof using.
+  intros e v Hev Hg.
+  hnf. autounfold with certiclasses eval in *. repnd.
+  dands; eauto with eval typeclass_instances.
+Qed.
+
+(* all variants of the correctness property need this part *)
+Lemma goodPres45 : goodPreserving (ienv * L4_5_Term) (ienv * L5Term).
+Proof using.
+  simpl. red. intros ? Hgood.
   unfold certiClasses.translate, liftTotal, bigStepEval,
   liftBigStepException, translateT, certiL4_5_to_L5. simpl.
   simpl. hnf. simpl.
   unfold goodTerm, dummyEnvWf, goodTerm, GoodTerm_instance_1, isprogram, closed in Hgood.
   destruct s as [? s]; simpl in *. repnd.
   hnf. simpl. symmetry. rewrite cps_cvt_aux_fvars; auto. rewrite Hgood2. refl.
+Qed.
+
+Global Instance certiL4_5_to_L5Correct: CerticoqTranslationCorrect certiL4_5 certiL5.
+(* Again, proof by induction *)
+Proof.
+  constructor.
+- exact goodPres45.
 - red. intros ? ? Hgood Heval.
   destruct Heval as [Heq Heval].
   destruct s as [senv s].
@@ -517,3 +541,186 @@ Check  @cps_cvt_corr.
      : exception (cTerm certiL5a)
 *)
 
+
+Require Import Common.certiClasses3.
+
+Section Temp.
+
+  Local Instance L4_5bs : BigStepOpSem (prod ienv L4_5_Term).
+  apply dummyEnvBigStep. eauto with typeclass_instances.
+  Defined.
+  Local Instance L5bs : BigStepOpSem (prod ienv (@NTerm NVar L5Opid)).
+  apply dummyEnvBigStep. eauto with typeclass_instances.
+  Defined.
+
+
+Local Instance L4_5MkApply : MkApply  (ienv * L4_5_Term) :=
+    fun f a => let (senv,f) := f in let (_, a) := a in (senv, App_e f a).
+
+  Definition extractL5Core (t:L5Term) :=
+    match t with
+      (*  L4_5_to_L5.Ret_c core haltCont => core *)
+      oterm CRet [bterm [] core; _] => core
+      | _ => oterm CRet [] (* impossible, hence garbage *)
+    end.
+
+  Local Instance L5MkApply : MkApply  (ienv * L5Term) :=
+    fun f a => let (senv,f) := f in
+            let (_, a) := a in
+            let a := extractL5Core a in
+            (senv, mkAppHalt (val_outer f) a).
+  
+  (*TODO: re add after ending sections *)
+
+  Hint Unfold L5bs  bigStepEval : certiclasses.
+
+  Require Import L4_5_to_L5.
+  (* Move *)
+  
+Lemma evalc_terminal
+     : forall e v,
+      eval_c e v -> eval_c v v.
+Proof using.
+  intros ? ? Heval.
+  induction Heval; auto;[]. (* eval_halt_c case. fix. require some kind of an is_value.
+A ugly hacky way would be to require that it is the vps_cvt_val of something. *)
+Admitted.
+
+(* this is not true. the argument of Halt_c may be anything *)
+Lemma evalc_halt
+     : forall hv v,
+      eval_c (Halt_c hv) v <-> eval_c hv v.
+Proof using.
+  intros.
+  split; intros Hyp.
+  - inversion Hyp. subst. eapply evalc_terminal; eauto.
+  - (* need the is_value hyp? *)
+
+Abort.    
+  
+Lemma goodSubterms25 : forall o lbt,
+    @goodTerm L4_5_Term _ (oterm o lbt)
+    -> forall nt, In (bterm [] nt) lbt  -> goodTerm nt.
+Proof using.
+  intros ? ? Hg ? Hin. autounfold with certiclasses eval in *.
+  unfold closed in *. simpl in *.
+  repnd.
+  rewrite  list.flat_map_empty in Hg2.
+  autorewrite with SquiggleEq in Hg0.
+  specialize (Hg2 _ Hin).
+  simpl in *.
+  dands; auto.
+  - intros ? Hc. apply Hg0. apply in_flat_map. eexists; dands; eauto.
+  - ntwfauto.
+  - rewrite Bool.andb_true_iff in Hg. apply proj2 in Hg.
+    rewrite list.ball_true in Hg. apply Hg.
+    apply in_map_iff. eexists; dands; eauto. reflexivity.
+Qed.    
+
+Lemma obsLinkableL45: compObsPreservingLinkable  (ienv * L4_5_Term) (ienv * L5Term).
+Proof.
+  intros ?.
+  revert s.
+  cofix.
+  intros ? Hgood.
+  constructor. constructor.
+  intros ? Heval.
+  simpl.
+  destruct Heval as [Heq Heval].
+  destruct s as [senv s].
+  destruct sv as [? sv]. symmetry in Heq.
+  simpl in *. subst.
+  exists (senv, (cps_cvt_val sv)).
+  pose proof (evalPreservesGood _ _ Heval Hgood) as Hgoodsv.
+  pose proof (eval_yields_value' _ _ Heval) as Hvalue.
+  repeat progress autounfold with certiclasses.
+  simpl in *. 
+  dands; [ reflexivity | | | | ].
+
+  + simpl in Hgood. autounfold with certiclasses in Hgood. simpl in Hgood.
+    simpl in Hgood. autounfold with certiclasses in Hgood. simpl in Hgood.
+    repnd.
+    destruct Hgood1 as [Hclosed Hwf].
+    rename Hgood0 into Hvc. rename Hgood into Hfixwf.    pose proof
+         (cps_cvt_corr _ _ Hwf Hfixwf Hvc Heval
+                       Hclosed haltCont
+                       eq_refl
+                       ((cps_cvt_val sv)))
+      as Hcps.
+    apply Hcps. clear Hcps.
+    hnf in Heval.
+    rewrite (cps_val_ret_flip sv); try split; eauto with eval typeclass_instances.
+    unfold haltCont.
+    apply haltContAp.
+  + hnf in Heval. apply eval_yields_value' in Heval.
+    revert Heval. clear. intros Hisv.
+    let tac := compute; intros qn;  destruct qn; constructor in
+    induction Hisv; simpl; [tac | tac |  | tac].
+    unfold yesPreserved, questionHead, QuestionHeadTermL45, QuestionHeadTermL5; cbn.
+    destruct q; auto. unfold implb. btauto.
+  + clear dependent s. intros n.
+    unfold yesPreserved, questionHead, QuestionHeadTermL45, QuestionHeadTermL5; cbn.
+    inversion Hvalue;
+    (* Not induction. Even though the arguments of constructors are all values, 
+     they may be lambdas, and after application, they may need computation *)
+    simpl; try (clear obsLinkableL45; compute; constructor; fail). subst.
+    repeat rewrite List.map_map.
+    repeat rewrite nth_error_map.
+    remember (List.nth_error es n) as esso.
+    destruct esso as [ess | ]; try constructor.
+    specialize (obsLinkableL45 (senv, ess)).
+    symmetry in Heqesso. apply nth_error_In in Heqesso.
+    assert (ident : goodTerm (senv, ess)) by
+      (eapply goodSubterms25;[apply Hgoodsv | apply in_map; assumption]).
+    specialize (obsLinkableL45 ident).
+    invertsn obsLinkableL45.
+    unfold translateT, certiL4_5_to_L5 in obsLinkableL45.
+    simpl in *.
+    revert obsLinkableL45.
+    assert (Hp:forall A B, (A<->B)->(A->B)) by tauto.
+    apply Hp. clear Hp.
+    apply compObsLeLinkRespectsSameVal;[ reflexivity | ].
+    intros ?.
+    apply and_iff_compat_l.
+    simpl.  unfold haltCont.
+    repeat (autounfold with certiclasses eval in ident;  simpl in ident). repnd.
+    rewrite (cps_val_ret_flip ess); unfold isprogram; eauto; try reflexivity.
+    simpl.
+    rewrite eval_ret. simpl. unfold subst. simpl.
+    admit. (* need a fix to L4_5_to_L5.eval_c, as indicated in comments there *)
+  + intros Hq ? Hga. unfold mkApp, L4_5MkApply, L5MkApply. simpl.
+    destruct svArg as [clear  svArg]. simpl. hnf in Hga. simpl in *. clear clear.
+    specialize (obsLinkableL45 (senv, App_e sv svArg)).
+    assert (ident : goodTerm (senv, App_e sv svArg)) by admit. (* app preserves goodness *)
+    specialize (obsLinkableL45 ident).
+    invertsn obsLinkableL45.
+    unfold translateT, certiL4_5_to_L5 in obsLinkableL45.
+    simpl in *. unfold mkAppHalt. unfold cps_cvt_apply in obsLinkableL45.
+    constructor.
+    revert obsLinkableL45.
+    assert (Hp:forall A B, (A<->B)->(A->B)) by tauto.
+    apply Hp. clear Hp.
+    apply compObsLeLinkRespectsSameVal;[ reflexivity | ].
+    unfold sameValues. intros v.
+    apply and_iff_compat_l.
+    simpl.  rewrite eval_ret. simpl.
+    assert (forall (l1 l2 r: L5Term), l1=l2 -> (eval_c l1 r <-> eval_c l2 r)) as Hp by (intros;subst;tauto).
+    apply Hp. clear Hp.
+    unfold subst. change_to_ssubst_aux8; [ | apply list.disjoint_nil_r ].
+    Local Transparent ssubst_aux ssubst_bterm_aux sub_filter.
+    autounfold with certiclasses in Hgoodsv.
+    unfold isprogram, closed in *.
+    assert (free_vars (cps_cvt sv) = []) as Hs.
+      (symmetry; rewrite cps_cvt_aux_fvars ; repnd; auto).
+    assert (free_vars (cps_cvt svArg) = []) as Hsa by
+      (symmetry; rewrite cps_cvt_aux_fvars ; repnd; auto; congruence).
+    simpl.
+    rewrite (fst ssubst_aux_trivial5) at 1; [ | simpl; rewrite Hs; apply list.disjoint_nil_l ].
+    rewrite (fst ssubst_aux_trivial5); [ | simpl; rewrite Hsa; apply list.disjoint_nil_l ].
+    unfold cps_cvt_apply_aux,  L4_5_to_L5.Ret_c,  L4_5_to_L5.KLam_c.
+    repeat f_equal.
+    apply cps_val_outer. apply is_valueb_corr. eapply eval_yields_value'; eauto.
+    Fail idtac.
+Abort.
+
+  End Temp.
